x86/Asmgenproof.v
@@ -654,6 +654,12 @@ Proof.
   exists (l++instr::nil). rewrite H. rewrite app_ass. simpl. auto.
 Qed.
 
+(* copy from Asmgenproof0.v *)
+Lemma parent_ra_type: forall s, match_stack s -> Val.has_type (parent_ra s) Tptr.
+Proof.
+  induction 1; simpl.
+  unfold Vnullptr; unfold Tptr; destruct Archi.ptr64; simpl; auto. inv H0. constructor.
+Qed.
 
 (** This is the simulation diagram.  We prove it by case analysis on the Mach transition. *)
 
